

By flux quantization

$$\vartheta_L - \vartheta_R + \phi = 0. \quad (*)$$

If $\vartheta_L = \vartheta + \phi/2$, then by (*) we have that

$$\begin{aligned} \vartheta_R &= \vartheta + 3\phi/2 \\ &\neq \vartheta + \frac{1}{2}\phi. \end{aligned}$$

If instead we define ϑ by

$$\vartheta \equiv \vartheta_L + \phi/2$$

$$\Rightarrow \vartheta = (\vartheta_L + \vartheta_R)/2 \quad \text{by } (*).$$


Using $\vartheta_L = \vartheta - \phi/2$ &

$$\vartheta_R = \vartheta + \phi/2,$$

the total current is given by

$$I = I_L \sin(\vartheta - \phi/2) + I_R \sin(\vartheta + \phi/2) \quad (\Delta)$$

Differentiating w.r.t. ϕ , one finds that

next
page 

$$\frac{dI}{d\phi} = \frac{1}{2} \left\{ -I_L \cos(s - \phi/2) + I_R \cos(s + \phi/2) \right\}$$

$$= \frac{1}{2} \left\{ \underline{I_R} \cos s \cos \phi/2 - \underline{I_R} \sin s \sin \phi/2 \right. \\ \left. - \underline{I_L} \cos s \cos \phi/2 - \underline{I_L} \sin s \sin \phi/2 \right\}$$

$$= \frac{1}{2} \left\{ (I_R - I_L) \cos s \cos \phi/2 \right. \\ \left. - (I_R + I_L) \sin s \sin \phi/2 \right\} \quad (1)$$

$$I = 0 \Rightarrow I_L \sin(s - \phi/2) = -I_R \sin(s + \phi/2)$$

or that

$$I_L (\sin s \cos \phi/2 - \cos s \sin \phi/2) \\ = -I_R (\sin s \cos \phi/2 + \cos s \sin \phi/2)$$

$$\Rightarrow (I_L + I_R) \sin s \cos \phi/2 = -(I_R - I_L) \cos s \sin \phi/2$$

$$\Rightarrow \sin \bar{\theta} = \frac{-(I_R - I_L)}{(I_R + I_L)} \frac{\cos \bar{\theta} \sin \phi/2}{\cos \phi/2} \quad (1)$$

Plugging (1) into (0), we have that

$$\frac{dI}{d\phi} = \frac{1}{2} \left\{ (I_R - I_L) \cos \bar{\theta} \cos \phi/2 + (I_R - I_L) \frac{\cos \bar{\theta} \sin \phi/2}{\cos \phi/2} \right\}$$

evaluating @ $\sin(\bar{\theta}) = 0$ and $\cos(\bar{\theta}) = 1$

$$\Rightarrow \left. \frac{dI}{d\phi} \right|_{\bar{\theta} = \bar{\theta}} = \frac{1}{2} (I_R - I_L) \left\{ \cos \phi/2 + \tan(\phi/2) \right\}$$